deps/poulet4/lib/P4automata/PreBisimulationSyntax.v
@@ -110,9 +110,9 @@ Section ConfRel.
   Context `{S_finite: @Finite S _ S_eq_dec}.
 
   (* Header identifiers. *)
-  Variable (H: Type).
-  Context `{H_eq_dec: EquivDec.EqDec H eq}.
-  Context `{H_finite: @Finite H _ H_eq_dec}.
+  Variable (H: nat -> Type).
+  Context `{H_eq_dec: forall n, EquivDec.EqDec (H n) eq}.
+  Context `{H_finite: @Finite (P4A.H' H) _ (P4A.H'_eq_dec (H_eq_dec:=H_eq_dec))}.
 
   Variable (a: P4A.t S H).
 
