deps/poulet4/lib/P4automata/Sum.v
@@ -23,10 +23,10 @@ Section Sum.
   Context `{S2_finite: @Finite S2 _ S2_eq_dec}.
 
   (* Header identifiers. *)
-  Variable (H1: Type).
-  Context `{H1_eq_dec: EquivDec.EqDec H1 eq}.
-  Variable (H2: Type).
-  Context `{H2_eq_dec: EquivDec.EqDec H2 eq}.
+  Variable (H1: nat -> Type).
+  Context `{H1_eq_dec: forall n, EquivDec.EqDec (H1 n) eq}.
+  Variable (H2: nat -> Type).
+  Context `{H2_eq_dec: forall n, EquivDec.EqDec (H2 n) eq}.
 
   Variable (a1: Syntax.t S1 H1).
   Variable (a2: Syntax.t S2 H2).
@@ -39,16 +39,19 @@ Section Sum.
   Global Instance S_finite: @Finite S _ S_eq_dec :=
     ltac:(typeclasses eauto).
 
-  Definition H : Type := H1 + H2.
+  Definition H (n: nat) : Type := H1 n + H2 n.
 
-  Global Instance H_eq_dec: EquivDec.EqDec H eq :=
+  Definition inl_ (n: nat) : H1 n -> H n := inl.
+  Definition inr_ (n: nat) : H2 n -> H n := inr.
+
+  Global Instance H_eq_dec: forall n, EquivDec.EqDec (H n) eq :=
     ltac:(typeclasses eauto).
 
   Program Definition sum : Syntax.t S H :=
     {| Syntax.t_states s :=
          match s with
-         | inl s1 => Syntax.state_fmapSH inl inl (a1.(Syntax.t_states) s1)
-         | inr s2 => Syntax.state_fmapSH inr inr (a2.(Syntax.t_states) s2)
+         | inl s1 => Syntax.state_fmapSH _ inl inl_ (a1.(Syntax.t_states) s1)
+         | inr s2 => Syntax.state_fmapSH _ inr inr_ (a2.(Syntax.t_states) s2)
          end |}.
   Next Obligation.
     destruct a1, a2, s;
